

# MAT1012

## Tutorial 10

CUHK(SZ)

April 8, 2024

# Outline

1 Tutorial Exercises

2 Midterm Solutions

**Ex.1.** Evaluate the integral

$$\iint_R f(x, y) dA,$$

where

$$f(x, y) = \begin{cases} 1, & y \leq e^x, \\ 0, & y > e^x, \end{cases}$$

and  $R = [0, 1] \times [0, e]$ .

Solution.

$$\begin{aligned}\iint_R f(x, y) dA &= \int_0^1 dx \int_0^e f(x, y) dy \\&= \int_0^1 \left( \int_0^{e^x} f(x, y) dy + \int_{e^x}^e f(x, y) dy \right) dx \\&= \int_0^1 \left( \int_0^{e^x} 1 dy + \int_{e^x}^e 0 dy \right) dx \\&= \int_0^1 dx \int_0^{e^x} dy = \int_0^1 e^x dx = e - 1.\end{aligned}$$



**Ex.2.** Evaluate the integral

$$\iint_D (e^{-x^2} + e^x \sin x) dx dy,$$

where  $D$  is the region enclosed by  $y = 0$ ,  $x = 1$  and  $y = x$ .

## Solution.

By the Fubini's theorem, we have

$$\begin{aligned}
 \iint_D (e^{-x^2} + e^x \sin x) dx dy &= \int_0^1 (e^{-x^2} + e^x \sin x) dx \int_0^x dy \\
 &= \int_0^1 (e^{-x^2} + e^x \sin x) x dx = \int_0^1 x e^{-x^2} dx + \frac{1}{2} \int_0^1 2x e^x \sin x dx \\
 &= -\frac{1}{2} e^{-x^2} \Big|_0^1 + \frac{1}{2} \left[ x e^x (\sin x - \cos x) \Big|_0^1 - \int_0^1 e^x (\sin x - \cos x) dx \right] \\
 &= \frac{1}{2} \left( 1 - \frac{1}{e} \right) + \frac{1}{2} e (\sin 1 - \cos 1) - \frac{1}{2} (-e^x \cos x) \Big|_0^1 \\
 &= \frac{1}{2} \left( 1 - \frac{1}{e} \right) + \frac{1}{2} e (\sin 1 - \cos 1) + \frac{1}{2} (e \cos 1 - 1) = \frac{e^2 \sin 1 - 1}{2e}.
 \end{aligned}$$

## Solution.

Here we used the fact

$$\begin{aligned}\int e^x(\sin x - \cos x)dx &= \int e^x \sin x dx - \int e^x \cos x dx \\ &= \int e^x \sin x dx - \left( e^x \cos x - \int e^x (-\sin x) dx \right) = -e^x \cos x + C.\end{aligned}$$



Remark.

The other iterated integral,

$$\int_0^1 dy \int_y^1 (e^{-x^2} + e^x \sin x) dx,$$

is hard to calculate directly.



**Ex.3.** Evaluate the integral

$$\iint_D \frac{x^2 - y^2}{\sqrt{x + y + 3}} dx dy,$$

where  $D = \{(x, y) : |x| + |y| \leq 1\}$ .

## Solution.

In the  $xy$ -plane, the region is

$$D = \{(x, y) : |x| + |y| \leq 1\}.$$

For the transformation

$$u(x, y) = x + y, \quad v(x, y) = x - y,$$

we have

$$\frac{\partial(u, v)}{\partial(x, y)} = \begin{vmatrix} 1 & 1 \\ 1 & -1 \end{vmatrix} = -2,$$

## Solution.

and the region corresponding to  $D$  in the  $uv$ -plane is

$$G = \{(u, v) : -1 \leq u \leq 1, \quad -1 \leq v \leq 1\}.$$

Since the substitution transformation is one-to-one with continuous first partial derivatives, it has an inverse transformation and there are equations  $u = \alpha(x, y)$ ,  $v = \beta(x, y)$  with continuous first partial derivatives transforming  $R$  back into  $G$ . Moreover, the Jacobian determinants of the transformations are related reciprocally by

$$\frac{\partial(x, y)}{\partial(u, v)} = \left( \frac{\partial(u, v)}{\partial(x, y)} \right)^{-1}. \quad (10)$$

## Solution.

From (10), we have

$$J = \frac{\partial(x, y)}{\partial(u, v)} = \left( \frac{\partial(u, v)}{\partial(x, y)} \right)^{-1} = -\frac{1}{2}.$$

Thus, we have

$$\begin{aligned} \iint_D \frac{x^2 - y^2}{\sqrt{x + y + 3}} dx dy &= \iint_G \frac{uv}{\sqrt{u + 3}} |J| du dv \\ &= \int_{-1}^1 \int_{-1}^1 \frac{uv}{2\sqrt{u + 3}} du dv = \frac{1}{2} \int_{-1}^1 \frac{u}{\sqrt{u + 3}} du \int_{-1}^1 v dv = 0. \end{aligned}$$

## Solution.

*Another Solution.*

Note that  $D = \{(x, y) : |x| + |y| \leq 1\}$ , and

$$\iint_D \frac{x^2}{\sqrt{x+y+3}} dx dy = \iint_D \frac{y^2}{\sqrt{y+x+3}} dy dx.$$

Thus, we have

$$\iint_D \frac{x^2 - y^2}{\sqrt{x+y+3}} dx dy = \iint_D \frac{x^2}{\sqrt{x+y+3}} dx dy - \iint_D \frac{y^2}{\sqrt{y+x+3}} dy dx = 0.$$



**Question 1** (35 marks). Let  $C$  be a curve given by

$$x = a \cos t, \quad y = a \sin t, \quad z = bt, \quad t \in \mathbb{R},$$

where  $a, b$  are positive constants.

(a) Find the unit tangent vector  $\mathbf{T}$ , the principal normal vector  $\mathbf{N}$ , and the curvature  $\kappa$  of the curve  $C$  for any  $t$ .

(b) Evaluate the integral

$$\int_0^\pi \mathbf{T}(t) \times \mathbf{N}(t) dt.$$

### Solution.

(a) The curve  $C$  can be represented by

$$\mathbf{r}(t) = a \cos t \mathbf{i} + a \sin t \mathbf{j} + bt \mathbf{k}.$$

Hence, we have

$$\mathbf{r}'(t) = -a \sin t \mathbf{i} + a \cos t \mathbf{j} + b \mathbf{k},$$

$$|\mathbf{r}'(t)| = \sqrt{a^2 \sin^2 t + a^2 \cos^2 t + b^2} = \sqrt{a^2 + b^2}.$$

## Solution.

Thus,

$$\mathbf{T} = \frac{\mathbf{r}'(t)}{|\mathbf{r}'(t)|} = \frac{1}{\sqrt{a^2 + b^2}}(-a \sin t \mathbf{i} + a \cos t \mathbf{j} + b \mathbf{k}),$$

$$\frac{d\mathbf{T}}{dt} = \frac{1}{\sqrt{a^2 + b^2}}(-a \cos t \mathbf{i} - a \sin t \mathbf{j}),$$

$$\left| \frac{d\mathbf{T}}{dt} \right| = \frac{a}{\sqrt{a^2 + b^2}},$$

$$\mathbf{N} = \frac{\frac{d\mathbf{T}}{dt}}{\left| \frac{d\mathbf{T}}{dt} \right|} = -\cos t \mathbf{i} - \sin t \mathbf{j},$$

$$\kappa = \left| \frac{d\mathbf{T}}{ds} \right| = \frac{\left| \frac{d\mathbf{T}}{dt} \right|}{\frac{ds}{dt}} = \frac{\left| \frac{d\mathbf{T}}{dt} \right|}{|\mathbf{r}'(t)|} = \frac{\frac{a}{\sqrt{a^2 + b^2}}}{\sqrt{a^2 + b^2}} = \frac{a}{a^2 + b^2}.$$



Proof.

(b)

$$\begin{aligned}\mathbf{T}(t) \times \mathbf{N}(t) &= \frac{1}{\sqrt{a^2 + b^2}} \begin{vmatrix} \mathbf{i} & \mathbf{j} & \mathbf{k} \\ -a \sin t & a \cos t & b \\ -\cos t & -\sin t & 0 \end{vmatrix} \\ &= \frac{1}{\sqrt{a^2 + b^2}} (b \sin t \mathbf{i} - b \cos t \mathbf{j} + a \mathbf{k}), \\ \int_0^\pi \mathbf{T}(t) \times \mathbf{N}(t) dt &= \frac{1}{\sqrt{a^2 + b^2}} \int_0^\pi (b \sin t \mathbf{i} - b \cos t \mathbf{j} + a \mathbf{k}) dt \\ &= \frac{1}{\sqrt{a^2 + b^2}} (-b \cos t \mathbf{i} - b \sin t \mathbf{j} + at \mathbf{k}) \Big|_{t=0}^{t=\pi} \\ &= \frac{1}{\sqrt{a^2 + b^2}} (2b \mathbf{i} + a\pi \mathbf{k}).\end{aligned}$$



**Question 2** (20 marks). Let

$$f(x, y) = \begin{cases} \frac{xy^2}{x^2+y^4}, & (x, y) \neq (0, 0), \\ 0, & (x, y) = (0, 0). \end{cases}$$

Examine continuity of  $f(x, y)$  at  $(0, 0)$  and prove your conclusion.

## Solution.

The function is not continuous at  $(0,0)$ . In fact the limit

$$\lim_{(x,y) \rightarrow (0,0)} \frac{xy^2}{x^2 + y^4}$$

does not exist.

To prove, take  $k > 0$  and consider the limit along the curve  $x = ky^2$ .

Then

$$\lim_{\substack{(x,y) \rightarrow (0,0), \\ x=ky^2}} \frac{xy^2}{x^2 + y^4} = \lim_{y \rightarrow 0} \frac{ky^4}{k^2y^4 + y^4} = \frac{k}{k^2 + 1},$$

which depends on  $k$ . Thus the limit does not exist, so the function is not continuous at  $(0,0)$ . □

**Question 3** (40 marks). Let

$$f(x, y) = \begin{cases} \frac{\sqrt[3]{x^4 - y^4}}{\sqrt[3]{x} + \sqrt[3]{y}} & \text{if } x \neq -y, \\ 0 & \text{if } x = -y. \end{cases}$$

- (a) Find  $\frac{\partial f}{\partial x}(0, 0)$  and  $\frac{\partial f}{\partial y}(0, 0)$ .
- (b) Find the directional derivative of  $f(x, y)$  at  $P(0, 0)$  along the direction  $\mathbf{u} = (\alpha, \beta)$ , where  $\alpha^2 + \beta^2 = 1$ .
- (c) Examine the differentiability of  $f(x, y)$  at  $P(0, 0)$  and prove your conclusion.

## Solution.

(a) If  $x \neq 0$ ,

$$f(x, 0) = \frac{\sqrt[3]{x^4}}{\sqrt[3]{x}} = \frac{x^{4/3}}{x^{1/3}} = x.$$

$$\frac{\partial f}{\partial x}(0, 0) = 1.$$

If  $y \neq 0$ ,

$$f(0, y) = \frac{\sqrt[3]{-y^4}}{\sqrt[3]{y}} = -\frac{y^{4/3}}{y^{1/3}} = -y.$$

$$\frac{\partial f}{\partial y}(0, 0) = -1.$$

## Solution.

(b) Note that  $f(0,0) = 0$ . Let  $\mathbf{u} = \alpha\mathbf{i} + \beta\mathbf{j}$ , where  $\alpha^2 + \beta^2 = 1$ .

If  $\alpha \neq -\beta$ , then  $\alpha s \neq -\beta s$  for any  $s > 0$ .

$$\begin{aligned}\frac{\partial f}{\partial \mathbf{u}}(0,0) &= \lim_{s \rightarrow 0^+} \frac{f(\alpha s, \beta s) - f(0,0)}{s} \\ &= \lim_{s \rightarrow 0^+} \frac{\sqrt[3]{(\alpha s)^4 - (\beta s)^4}}{s(\sqrt[3]{\alpha s} + \sqrt[3]{\beta s})} = \frac{\sqrt[3]{\alpha^4 - \beta^4}}{\sqrt[3]{\alpha} + \sqrt[3]{\beta}} = \frac{\sqrt[3]{\alpha^2 - \beta^2}}{\sqrt[3]{\alpha} + \sqrt[3]{\beta}}.\end{aligned}$$

In the last equality, since  $\alpha^2 + \beta^2 = 1$ ,

$$\alpha^4 - \beta^4 = (\alpha^2 - \beta^2)(\alpha^2 + \beta^2) = \alpha^2 - \beta^2.$$

If  $\alpha = -\beta$ , then  $\alpha s = -\beta s$  for any  $s > 0$ ,  $f(\alpha s, \beta s) = 0$ , so

$$\frac{\partial f}{\partial \mathbf{u}}(0,0) = 0.$$

## Solution.

(c) The function  $f$  is not differentiable at  $P(0, 0)$ . Otherwise we have, for  $\mathbf{u} = \alpha\mathbf{i} + \beta\mathbf{j}$  with  $\alpha^2 + \beta^2 = 1$ ,

$$\frac{\partial f}{\partial \mathbf{u}}(0, 0) = \nabla f(0, 0) \cdot \mathbf{u} = (1, -1) \cdot (\alpha, \beta) = \alpha - \beta.$$

This is not true if  $\alpha = -\beta$ .

**Direct proof.** Suppose  $f$  is differentiable at  $P(0, 0)$ , then

$$f(x, y) - f(0, 0) - f_x(0, 0)x - f_y(0, 0)y = o(\rho)$$

as  $\rho \rightarrow 0$ , where  $\rho = \sqrt{x^2 + y^2}$ . So

$$f(x, y) - x + y = o(\rho).$$

## Solution.

However, along  $x = 2t$ ,  $y = t$ ,  $t > 0$ , we have

$$f(x, y) = f(2t, t) = \frac{\sqrt[3]{16t^4 - t^4}}{\sqrt[3]{2t} + \sqrt[3]{t}} = \frac{\sqrt[3]{15}t^{4/3}}{(\sqrt[3]{2} + 1)t^{1/3}} = \frac{\sqrt[3]{15}}{\sqrt[3]{2} + 1}t,$$

$$f(x, y) - x + y = f(2t, t) - 2t + t = f(2t, t) - t = \left(\frac{\sqrt[3]{15}}{\sqrt[3]{2} + 1} - 1\right)t$$

$$\rho = \sqrt{x^2 + y^2} = \sqrt{4t^2 + t^2} = \sqrt{5}t.$$

Since

$$\frac{f(x, y) - x + y}{\rho} = \frac{\left(\frac{\sqrt[3]{15}}{\sqrt[3]{2} + 1} - 1\right)t}{\sqrt{5}t} = \frac{\left(\frac{\sqrt[3]{15}}{\sqrt[3]{2} + 1} - 1\right)}{\sqrt{5}}$$

which does not tend to zero as  $t \rightarrow 0^+$ , we reach a contradiction. Thus,  $f$  is not differentiable at  $(0, 0)$ . □



**Question 4** (15 marks). Let  $f(x, y)$  be a continuous function defined on the plane and assume

$$\lim_{|x|+|y|\rightarrow\infty} f(x, y) = -\infty.$$

Prove that  $f$  attains its maximum value.

## Solution.

Since  $\lim_{|x|+|y|\rightarrow\infty} f(x,y) = -\infty$ , there exists  $R > 0$  such that

$$f(x,y) < f(0,0)$$

if  $|x| + |y| \geq R$ . The set

$$D = \{(x,y) \in \mathbb{R}^2 : |x| + |y| \leq R\}$$

is a bounded and closed set. Let

$$M = \sup_{(x,y) \in D} f(x,y).$$

Then  $f(0,0) \leq M$ , hence for any  $(x,y) \notin D$  we have  $f(x,y) < M$ .

## Solution.

Hence

$$M = \sup_{(x,y) \in \mathbb{R}^2} f(x,y).$$

By the definition of supremum, there exists  $(x_n, y_n) \in D$  such that  $f(x_n, y_n) \rightarrow M$ . Since  $D$  is bounded, so  $\{(x_n, y_n)\}$  is bounded, hence there exists a subsequence  $\{(x_{n_j}, y_{n_j})\} \rightarrow (x_0, y_0)$ . Since  $f$  is continuous,

$$f(x_0, y_0) = \lim_{j \rightarrow \infty} f(x_{n_j}, y_{n_j}) = M.$$

Thus  $f$  achieves the maximum at  $(x_0, y_0)$ . □

**Question 5** (25 marks). Find the set of convergence of the series

$$\sum_{n=1}^{\infty} \frac{\ln(1+nx)}{n} (\sin x)^n, \quad x \geq 0,$$

### Solution.

The set of convergence is

$$\begin{aligned} D &= \{x \geq 0 : x \neq 2k\pi + \frac{\pi}{2} \text{ for any integer } k \geq 0\} \\ &= [0, \infty) \setminus \bigcup_{k=0}^{\infty} \{2k\pi + \frac{\pi}{2}\}. \end{aligned}$$

The series converges at  $x = 0$ .

## Solution.

Let  $x > 0$ . Denote  $u_n(x) = \frac{\ln(1+nx)}{n}(\sin x)^n$ . Note that

$$\begin{aligned}\ln(1 + (n+1)x) &= \ln((1+nx) + x) = \ln[(1+nx)1 + \frac{x}{1+nx}] \\ &= \ln(1+nx) + \ln(1 + \frac{x}{1+nx}).\end{aligned}$$

$$\begin{aligned}\frac{u_{n+1}(x)}{u_n(x)} &= \frac{\frac{\ln(1+(n+1)x)}{n+1}(\sin x)^{n+1}}{\frac{\ln(1+nx)}{n}(\sin x)^n} = \frac{n}{n+1} \sin x \frac{\ln(1+nx) + \ln(1 + \frac{x}{1+nx})}{\ln(1+nx)} \\ &= \frac{n}{n+1} \sin x \left[1 + \frac{\ln(1 + \frac{x}{1+nx})}{\ln(1+nx)}\right] \rightarrow \sin x\end{aligned}$$

as  $n \rightarrow \infty$ . By the ratio test the series converges if  $|\sin x| < 1$ , namely if  $x > 0$ ,  $x \neq k\pi + \frac{\pi}{2}$  for any integer  $k \geq 0$ .

## Solution.

If  $x = 2k\pi + \frac{\pi}{2}$ , then  $\sin x = 1$ , then  $u_n(x) = \frac{\ln(1+nx)}{n} > \frac{1}{n}$  for large  $n$ .

By comparison test the series diverges.

If  $x = (2k+1)\pi + \frac{\pi}{2}$ , then  $\sin x = -1$ , the series is

$$\sum_{n=1}^{\infty} (-1)^n \frac{\ln(1+nx)}{n},$$

which is an alternating series. We show the sequence  $a_n = \frac{\ln(1+nx)}{n}$  decreases to zero as  $n \rightarrow \infty$ .

## Solution.

Fix  $x > 0$  and consider the function

$$g(t) = \frac{\ln(1 + xt)}{t}.$$

$$g'(t) = \frac{1}{t^2} \left( \frac{tx}{1 + xt} - \ln(1 + xt) \right) < 0$$

because

$$\ln(1 + xt) > \frac{xt}{1 + xt}$$

for  $xt > 0$ . Hence  $a_n = g(n)$  is decreasing in  $n$ . Obviously  $a_n \rightarrow 0$  as  $n \rightarrow \infty$ . By Lebnitz test we conclude that  $\sum_{n=1}^{\infty} (-1)^n a_n$  converges.  $\square$



**Question 6** (20 marks). Let  $\{a_n\}$  be a sequence of positive numbers. Assume there exists  $p > 0$  such that

$$\lim_{n \rightarrow \infty} \frac{\ln(na_n)}{\ln(\ln n)} = -p. \quad (*)$$

- (a) Prove that if  $p > 1$  then the series  $\sum_{n=3}^{\infty} a_n$  converges, and if  $0 < p < 1$  then  $\sum_{n=1}^{\infty} a_n$  diverges.
- (b) Can you conclude the series converges or diverges if  $p = 1$ ? Give your reason.

## Solution.

(a) From (\*), for any  $0 < \varepsilon < p$ , there exists  $N$  such that for any  $n \geq N$ ,

$$p - \varepsilon < -\frac{\ln(na_n)}{\ln \ln n} < p + \varepsilon,$$

$$\ln((\ln n)^{p-\varepsilon}) = (p - \varepsilon) \ln \ln n < -\ln(na_n) < (p + \varepsilon) \ln \ln n = \ln((\ln n)^{p+\varepsilon}),$$

$$-\ln((\ln n)^{p+\varepsilon}) < \ln(na_n) < -\ln((\ln n)^{p-\varepsilon}),$$

$$\ln \frac{1}{(\ln n)^{p+\varepsilon}} < \ln(na_n) < \ln \frac{1}{(\ln n)^{p-\varepsilon}},$$

$$\frac{1}{(\ln n)^{p+\varepsilon}} < na_n < \frac{1}{(\ln n)^{p-\varepsilon}},$$

$$\frac{1}{n(\ln n)^{p+\varepsilon}} < a_n < \frac{1}{n(\ln n)^{p-\varepsilon}}.$$

## Solution.

If  $p > 1$ , we take  $\varepsilon > 0$  such that  $p - \varepsilon > 1$ . Since the series  $\sum_{n=N}^{\infty} \frac{1}{n(\ln n)^{p-\varepsilon}}$  converges and  $0 < a_n < \frac{1}{n(\ln n)^{p-\varepsilon}}$ , we conclude that  $\sum_{n=N}^{\infty} a_n$  converges.

If  $p < 1$ , we take  $\varepsilon > 0$  such that  $p + \varepsilon < 1$ . Since the series  $\sum_{n=N}^{\infty} \frac{1}{n(\ln n)^{p+\varepsilon}}$  diverges and  $a_n > \frac{1}{n(\ln n)^{p+\varepsilon}}$ , we conclude that  $\sum_{n=N}^{\infty} a_n$  diverges.

## Solution.

(b) No. Let

$$a_n = \frac{1}{n(\ln n)(\ln \ln n)^q}, \quad q > 0.$$

$$\ln(na_n) = -\ln[(\ln n)(\ln \ln n)^q] = -\ln \ln n - q \ln \ln \ln n,$$

$$\frac{\ln(na_n)}{\ln \ln n} = -1 - q \frac{\ln \ln \ln n}{\ln \ln n} \rightarrow -1.$$

The series  $\sum_{n=N}^{\infty} a_n$  converges if  $q > 1$  and diverges if  $0 < q \leq 1$ . □

**Question 7** (20 marks). Let  $\sum_{n=1}^{\infty} u_n(x)$  be a series of functions and  $\sum_{n=0}^{\infty} a_n x^n$  be a power series. Assume there exists a positive number  $c$  such that the following conditions hold:

- (1) Every  $u_n(x)$  is continuously differentiable on  $[0, c]$ .
- (2)  $|u_n(x)| \leq a_n c^n$  for all  $x \in [0, c]$  and  $n \geq 1$ .
- (3)  $|u'_n(x)| \leq n a_n x^{n-1}$  for all  $x \in (0, c)$  and  $n \geq 1$ .
- (4) The series  $\sum_{n=0}^{\infty} a_n x^n$  converges at  $x = c$ .

Prove the following conclusions:

- (a)  $\sum_{n=1}^{\infty} u_n(x)$  converges uniformly on the interval  $[0, c]$ .
- (b) Let  $f(x) = \sum_{n=1}^{\infty} u_n(x)$ . Then  $f$  is continuously differentiable in the open interval  $(0, c)$ .

## Solution.

By condition (4) the power series converges at  $x = c$ , hence it converges uniformly on  $[0, c]$  (see Exercise 4.3.8). From this and condition (2), we can use the M-test to conclude that the series  $\sum_{n=1}^{\infty} u_n(x)$  converges uniformly on  $[0, c]$ .

From (4) the radius of convergence of the power series  $R \geq c$ . Hence the radius of convergence of  $\sum_{n=1}^{\infty} na_n x^{n-1}$  is also  $R$ , thus it converges for  $|x| < c$ . Let  $x_0 \in (0, c)$ . For any  $|x_0| < b < c$  the series  $\sum_{n=1}^{\infty} na_n b^{n-1}$  converges. From (3), for all  $x \in (0, b]$  we have

$$|u'_n(x)| \leq na_n x^{n-1} \leq na_n b^{n-1}.$$

## Solution.

By the M-test we see that  $\sum_{n=1}^{\infty} u'_n(x)$  converges uniformly on  $(0, b]$ , hence we can differentiate the power series to get

$$f'(x) = \sum_{n=1}^{\infty} u'_n(x)$$

for  $x \in (0, b]$ . Since this power series converges uniformly on  $(0, b]$  and each  $u'_n(x)$  is continuous in  $(0, b]$  we see that  $f'(x)$  is continuous on  $(0, b]$ , in particular  $f'(x)$  is continuous at  $x_0$ . This is true for any  $x \in (0, c)$ , so we conclude that  $f'$  is continuous on  $(0, c)$ . □

**Question 8** (25 marks). Let  $f(x, y)$  be a function defined on an open disc  $B(x_0, y_0, R)$  with center  $P_0(x_0, y_0)$  and radius  $R > 0$ .

(a) Prove that if  $f$  is differentiable at  $P_0(x_0, y_0)$ , then the following conclusions hold:

(a1) For any unit vector  $\mathbf{u} = u_1\mathbf{i} + u_2\mathbf{j}$ , and for any smooth curve

$$\begin{cases} x = x(t), & y = y(t), & -1 \leq t \leq 1, \\ x(0) = x_0, & y(0) = y_0, & x'(0) = u_1, & y'(0) = u_2, \end{cases} \quad (1)$$

it holds that  $\left(\frac{d}{dt}\right)_+ f(x(t), y(t))\Big|_{t=0} = \frac{\partial f}{\partial \mathbf{u}}(x_0, y_0)$ , (2)

where  $\frac{\partial f}{\partial \mathbf{u}}(x_0, y_0)$  denotes the directional derivative of  $f$  at  $P_0(x_0, y_0)$  along the direction  $\mathbf{u}$ .

(a2)  $\frac{\partial f}{\partial \mathbf{u}}(x_0, y_0)$  is continuous in  $\mathbf{u}$ .



## Midterm Solutions

(b) Assume  $f$  has directional derivative  $\frac{\partial f}{\partial \mathbf{u}}(x_0, y_0)$  for all unit vector  $\mathbf{u}$ , and assume  $\frac{\partial f}{\partial \mathbf{u}}(x_0, y_0)$  is continuous in  $\mathbf{u}$ .

(b1) Can you conclude that  $f$  is differentiable at  $P_0(x_0, y_0)$ ?

(b2) Can you conclude that the equality (2) still holds true?

For each of (b1) and (b2), if your answer is “YES” then give a proof; if your answer is “NO” then give a counterexample.

### Solution.

(a1) Assume  $f$  is differentiable at  $(x_0, y_0)$ , there exists  $\delta > 0$  such that

$$\begin{aligned} f(x, y) = & f(x_0, y_0) + f_x(x_0, y_0)(x - x_0) + f_y(x_0, y_0)(y - y_0) \\ & + \varepsilon_1(x - x_0) + \varepsilon_2(y - y_0) \end{aligned} \quad (3)$$

whenever  $|x - x_0|^2 + |y - y_0|^2 < \delta^2$ , where  $\varepsilon_1, \varepsilon_2 \rightarrow 0$  as both  $x - x_0, y - y_0 \rightarrow 0$ .

## Solution.

For any unit vector  $\mathbf{u} = u_1\mathbf{i} + u_2\mathbf{j}$ , and any smooth curve satisfying (1), we have

$$x(t) = x_0 + u_1t + o(t), \quad y(t) = y_0 + u_2t + o(t).$$

Plugging  $x = x(t)$  and  $y = y(t)$  into (3) we get

$$\begin{aligned} & f(x(t), y(t)) - f(x_0, y_0) \\ &= f_x(x_0, y_0)[u_1t + o(t)] + f_y(x_0, y_0)[u_2t + o(t)] \\ & \quad + \varepsilon_1(x(t) - x_0) + \varepsilon_2(y(t) - y_0) \\ &= [f_x(x_0, y_0)u_1 + f_y(x_0, y_0)u_2]t + o(t) + \varepsilon_1(x(t) - x_0) + \varepsilon_2(y(t) - y_0). \end{aligned}$$

## Solution.

Hence

$$\begin{aligned} \left( \frac{d}{dt} \right)_+ f(x(t), y(t)) \Big|_{t=0} &= \lim_{t \rightarrow 0^+} \frac{f(x(t), y(t)) - f(x_0, y_0)}{t} \\ &= \lim_{t \rightarrow 0^+} \left\{ [f_x(x_0, y_0)u_1 + f_y(x_0, y_0)u_2] \right. \\ &\quad \left. + \frac{o(t) + \varepsilon_1(x(t) - x_0) + \varepsilon_2(y(t) - x_0)}{t} \right\} \\ &= f_x(x_0, y_0)u_1 + f_y(x_0, y_0)u_2 \\ &= \nabla f(x_0, y_0) \cdot \mathbf{u} = \frac{\partial f}{\partial \mathbf{u}}(x_0, y_0). \end{aligned}$$

### Solution.

Here we used the fact that as  $t \rightarrow 0^+$ ,

$$\Delta x = x(t) - x_0 \rightarrow 0, \quad \Delta y = y(t) - y_0 \rightarrow 0,$$

hence  $\varepsilon_1 \rightarrow 0$  and  $\varepsilon_2 \rightarrow 0$ . We also used the fact that since  $f$  is differentiable at  $(x_0, y_0)$ , the directional derivative  $\frac{\partial f}{\partial \mathbf{u}}(x_0, y_0)$  exists and it is equal to  $\nabla f(x_0, y_0) \cdot \mathbf{u}$ . Therefore the directional derivative exists and (2) holds.

## Solution.

(a2) Since  $f$  is differentiable at  $(x_0, y_0)$ , for any unit vector  $\mathbf{u}$  we have

$$\frac{\partial f}{\partial \mathbf{u}}(x_0, y_0) = \nabla f(x_0, y_0) \cdot \mathbf{u}.$$

If  $\mathbf{u}_j = \alpha_j \mathbf{i} + \beta_j \mathbf{j}$  are unit vectors, then

$$\begin{aligned} \left| \frac{\partial f}{\partial \mathbf{u}_1}(x_0, y_0) - \frac{\partial f}{\partial \mathbf{u}_2}(x_0, y_0) \right| &= |\nabla f(x_0, y_0) \cdot \mathbf{u}_1 - \nabla f(x_0, y_0) \cdot \mathbf{u}_2| \\ &= |\nabla f(x_0, y_0) \cdot (\mathbf{u}_1 - \mathbf{u}_2)| = |f_x(x_0, y_0)(\alpha_1 - \alpha_2) + f_y(x_0, y_0)(\beta_1 - \beta_2)| \\ &\leq \sqrt{f_x(x_0, y_0)^2 + f_y(x_0, y_0)^2} \sqrt{(\alpha_1 - \alpha_2)^2 + (\beta_1 - \beta_2)^2} \\ &= |\nabla f(x_0, y_0)| |\mathbf{u}_1 - \mathbf{u}_2|. \end{aligned}$$

### Solution.

Thus for any  $\varepsilon > 0$ , if  $\mathbf{u}_1, \mathbf{u}_2$  are unit vectors and

$$|\mathbf{u}_1 - \mathbf{u}_2| < \frac{\varepsilon}{1 + |\nabla f(x_0, y_0)|},$$

then

$$\left| \frac{\partial f}{\partial \mathbf{u}_1}(x_0, y_0) - \frac{\partial f}{\partial \mathbf{u}_2}(x_0, y_0) \right| < \varepsilon.$$

Thus  $\frac{\partial f}{\partial \mathbf{u}}(x_0, y_0)$  is continuous in  $\mathbf{u}$ .

## Solution.

(b) Assume  $f$  has directional derivative  $\frac{\partial f}{\partial \mathbf{u}}(x_0, y_0)$  for all unit vector  $\mathbf{u}$  and  $\frac{\partial f}{\partial \mathbf{u}}(x_0, y_0)$  is continuous in  $\mathbf{u}$ , we can not conclude  $f$  is differentiable at  $P_0(x_0, y_0)$ , we can not conclude (2) holds.

(b1) We can not conclude  $f$  is differentiable at  $P_0(x_0, y_0)$ .

Counterexample:

$$f(x, y) = \begin{cases} \frac{x^2 y}{x^2 + y^2}, & (x, y) \neq (0, 0), \\ 0, & (x, y) = (0, 0), \end{cases}$$

$$\nabla f(0, 0) = (0, 0).$$



### Solution.

For any unit vector  $\mathbf{u} = (\alpha, \beta)$ ,

$$f(\alpha t, \beta t) = \alpha^2 \beta t, \quad \frac{\partial f}{\partial \mathbf{u}}(0, 0) = \alpha^2 \beta,$$

which is continuous in  $(\alpha, \beta)$ , hence continuous in  $\mathbf{u}$ . Hence the directional derivative exists for any unit vector  $\mathbf{u}$  and is continuous in  $\mathbf{u}$ .

But  $f$  is not differentiable at  $P_0(0, 0)$ .

## Solution.

To prove, suppose  $f$  is differentiable at  $P_0(0,0)$ . Since  $f(0,0) = f_x(0,0) = f_y(0,0) = 0$ , we have, for  $(x,y) \neq (0,0)$ ,

$$\frac{x^2y}{x^2+y^2} = f(x,y) = \varepsilon_1x + \varepsilon_2y,$$

where  $\varepsilon_1, \varepsilon_2 \rightarrow 0$  as  $(x,y) \rightarrow (0,0)$ . Take  $y = x$ . We have

$$x = (\varepsilon_1 + \varepsilon_2)x,$$

$$1 = \varepsilon_1 + \varepsilon_2,$$

which is a contradiction.

## Solution.

**Other counterexample:**

$$f(x, y) = \begin{cases} 1, & 0 < y < x^2, \\ 0, & \text{otherwise.} \end{cases}$$

At  $P_0 = (0, 0)$ ,  $f$  has directional derivative in any direction  $\mathbf{u}$  and for any  $\mathbf{u}$

$$\frac{\partial f}{\partial \mathbf{u}}(0, 0) = 0.$$

Hence  $\frac{\partial f}{\partial \mathbf{u}}(0, 0)$  is continuous in  $\mathbf{u}$ . See PPT-Lecture 21, Example 5.4.15 (c).  $f$  is not continuous at  $P_0$ , hence  $f$  is not differentiable at  $P_0$ .

## Solution.

(b2) We can not conclude (2) holds. Counterexample:

$$f(x, y) = \begin{cases} x + y, & 0 < y < x^2, \\ 0, & \text{otherwise.} \end{cases}$$

Given any unit vector  $\mathbf{u} = u_1\mathbf{i} + u_2\mathbf{j}$ , the line segment  $x = u_1t$  and  $y = u_2t$  does not lie in the region  $0 < y < x^2$  for small  $t > 0$ , so

$$f(u_1t, u_2t) = 0$$

for small  $t \geq 0$ . Hence we have again  $\frac{\partial f}{\partial \mathbf{u}}(0, 0) = 0$ . Thus  $\frac{\partial f}{\partial \mathbf{u}}(0, 0)$  exists for any unit  $\mathbf{u}$  and is continuous in  $\mathbf{u}$ .

### Solution.

In particular if  $\mathbf{u} = \mathbf{i}$ , then  $\frac{\partial f}{\partial \mathbf{u}}(0, 0) = 0$ .

However if we choose the curve

$$x(t) = t, \quad y(t) = t^3, \quad -1 \leq t \leq 1,$$

then  $x(0) = 0$ ,  $y(0) = 0$ .  $x'(0) = 1$ ,  $y'(0) = 0$ , hence the curve has tangent vector  $\mathbf{u} = \mathbf{i}$  at  $t = 0$ . However the curve satisfies  $0 < y(t) < x^2(t)$  for all  $0 < t < 1$ .

## Solution.

Hence

$$f(x(t), y(t)) = x(t) + y(t) = t + t^3, \quad 0 \leq t < 1.$$

Hence

$$\left(\frac{d}{dt}\right)f(x(t), y(t))\Big|_{t=0} = \left(\frac{d}{dt}\right)\Big|_{t=0}(t + t^3) = 1 \neq \frac{\partial f}{\partial \mathbf{u}}(0, 0).$$

